theories/concurrent/ws_deque.v
@@ -42,41 +42,46 @@ Record ws_deque `{!heapGS Σ} {unboxed : bool} := {
   ws_deque_make_spec ι :
     {{{ True }}}
       ws_deque_make #()
-    {{{ t γ, RET t; ws_deque_inv t γ ι ∗ ws_deque_model t γ [] ∗ ws_deque_owner t γ }}} ;
+    {{{ t γ,
+      RET t;
+      ws_deque_inv t γ ι ∗
+      ws_deque_model t γ [] ∗
+      ws_deque_owner t γ
+    }}} ;
 
   ws_deque_push_spec t γ ι v :
     <<<
-      ws_deque_inv t γ ι ∗ ws_deque_owner t γ |
-      ∀∀ vs, ws_deque_model t γ vs
+      ws_deque_inv t γ ι ∗ ws_deque_owner t γ
+    | ∀∀ vs, ws_deque_model t γ vs
     >>>
       ws_deque_push t v @ ↑ι
     <<<
-      ws_deque_model t γ (vs ++ [v]) |
-      RET #(); ws_deque_owner t γ
+      ws_deque_model t γ (vs ++ [v])
+    | RET #(); ws_deque_owner t γ
     >>> ;
 
   ws_deque_pop_spec t γ ι :
     <<<
-      ws_deque_inv t γ ι ∗ ws_deque_owner t γ |
-      ∀∀ vs, ws_deque_model t γ vs
+      ws_deque_inv t γ ι ∗ ws_deque_owner t γ
+    | ∀∀ vs, ws_deque_model t γ vs
     >>>
       ws_deque_pop t @ ↑ι
     <<< ∃∃ o,
       (⌜vs = [] ∧ o = NONEV⌝ ∗ ws_deque_model t γ []) ∨
-      (∃ vs' v, ⌜vs = vs' ++ [v] ∧ o = SOMEV v⌝ ∗ ws_deque_model t γ vs') |
-      RET o; ws_deque_owner t γ
+      (∃ vs' v, ⌜vs = vs' ++ [v] ∧ o = SOMEV v⌝ ∗ ws_deque_model t γ vs')
+    | RET o; ws_deque_owner t γ
     >>> ;
 
   ws_deque_steal_spec t γ ι :
     <<<
-      ws_deque_inv t γ ι |
-      ∀∀ vs, ws_deque_model t γ vs
+      ws_deque_inv t γ ι
+    | ∀∀ vs, ws_deque_model t γ vs
     >>>
       ws_deque_steal t @ ↑ι
     <<< ∃∃ o,
       (⌜vs = [] ∧ o = NONEV⌝ ∗ ws_deque_model t γ []) ∨
-      (∃ v vs', ⌜vs = v :: vs' ∧ o = SOMEV v⌝ ∗ ws_deque_model t γ vs') |
-      RET o; True
+      (∃ v vs', ⌜vs = v :: vs' ∧ o = SOMEV v⌝ ∗ ws_deque_model t γ vs')
+    | RET o; True
     >>> ;
 
   ws_deque_unboxed :
