theories/concurrent/mpmc_stack.v
@@ -30,20 +30,33 @@ Record mpmc_stack `{!heapGS Σ} {unboxed : bool} := {
   mpmc_stack_make_spec ι :
     {{{ True }}}
       mpmc_stack_make #()
-    {{{ t γ, RET t; mpmc_stack_inv t γ ι ∗ mpmc_stack_model t γ [] }}} ;
+    {{{ t γ,
+      RET t;
+      mpmc_stack_inv t γ ι ∗
+      mpmc_stack_model t γ []
+    }}} ;
 
   mpmc_stack_push_spec t γ ι v :
-    <<< mpmc_stack_inv t γ ι | ∀∀ vs, mpmc_stack_model t γ vs >>>
+    <<<
+      mpmc_stack_inv t γ ι
+    | ∀∀ vs, mpmc_stack_model t γ vs
+    >>>
       mpmc_stack_push t v @ ↑ι
-    <<< mpmc_stack_model t γ (v :: vs) | RET #(); True >>> ;
+    <<<
+      mpmc_stack_model t γ (v :: vs)
+    | RET #(); True
+    >>> ;
 
   mpmc_stack_pop_spec t γ ι :
-    <<< mpmc_stack_inv t γ ι | ∀∀ vs, mpmc_stack_model t γ vs >>>
+    <<<
+      mpmc_stack_inv t γ ι
+    | ∀∀ vs, mpmc_stack_model t γ vs
+    >>>
       mpmc_stack_pop t @ ↑ι
     <<< ∃∃ o,
       (⌜vs = [] ∧ o = NONEV⌝ ∗ mpmc_stack_model t γ []) ∨
-      (∃ v vs', ⌜vs = v :: vs' ∧ o = SOMEV v⌝ ∗ mpmc_stack_model t γ vs') |
-      RET o; True
+      (∃ v vs', ⌜vs = v :: vs' ∧ o = SOMEV v⌝ ∗ mpmc_stack_model t γ vs')
+    | RET o; True
     >>> ;
 
   mpmc_stack_unboxed :
